@prefix rdf: <http://www.w3.org/1999/02/22-rdf-syntax-ns#> .
@prefix rdfs: <http://www.w3.org/2000/01/rdf-schema#> .
@prefix xsd: <http://www.w3.org/2001/XMLSchema#> .
@prefix xml: <http://www.w3.org/XML/1998/namespace> .
@prefix dc: <http://purl.org/dc/elements/1.1/#> .
@prefix owl: <http://www.w3.org/2002/07/owl#> .
@prefix owl2: <http://www.w3.org/2006/12/owl2#> .
@prefix swrlx: <http://www.w3.org/2003/11/swrlx#> .
@prefix event: <http://purl.org/NET/c4dm/event.owl#> .
@prefix time: <http://www.w3.org/2006/time#> .
@prefix foaf: <http://xmlns.com/foaf/0.1/> .

@prefix mere: <http://www.bbn.com/ontologies/domain/foundation/mereology#> .
@prefix tapio: <http://www.invincea.com/ontologies/icas/1.0/tapio#> .
@prefix user: <http://www.invincea.com/ontologies/icas/1.0/user#> .
@prefix filesystem: <http://www.invincea.com/ontologies/icas/1.0/filesystem#> .
@prefix : <http://www.invincea.com/ontologies/icas/1.0/acl#> .
@base <http://www.invincea.com/ontologies/icas/1.0/acl> .

<http://www.invincea.com/ontologies/icas/1.0/acl> 
			rdf:type owl:Ontology ;
			rdfs:label "Access Control List ontology"@en ;
		    rdfs:comment "an ontology of common access control settings."@en ;
		    dc:description "an ontology of common access control settings."@en ;
		    owl:versionInfo "1.0" ;
		    dc:creator: "Invincea Labs"@en ;
		    dc:date "2014" ;
		    owl:imports <http://www.invincea.com/ontologies/icas/1.0/user> .
			
:deniesExecuteTo 
			rdf:type owl:ObjectProperty ;
			rdfs:label "denies execution by"@en ;
			rdfs:comment "even if some other ACL would indirectly grant execution rights to this user or group, this ACL entry overrides that and explicitly forbids execution."@en ;
			rdfs:domain :ACLEntry ;
			rdfs:range user:Group , user:UserAccount , :default .

:deniesReadTo 
			rdf:type owl:ObjectProperty ;
		    rdfs:label "denies read by"@en ;
		    rdfs:comment "even if some other ACL would indirectly grant read rights to this user or group, this ACL entry overrides that and explicitly forbids reading."@en ;
		    rdfs:domain :ACLEntry ;
		    rdfs:range user:Group , user:UserAccount , :default .

:deniesWriteTo 
			rdf:type owl:ObjectProperty ;
		    rdfs:label "explicitly denies write by"@en ;
		    rdfs:comment "even if some other ACL would indirectly grant write rights to this user or group, this ACL entry overrides that and explicitly forbids writing."@en ;
		    rdfs:domain :ACLEntry ;
		    rdfs:range user:Group , user:UserAccount , :default .


:grantsExecuteTo 
			rdf:type owl:ObjectProperty ;
		    rdfs:label "grants execution by"@en ;
		    rdfs:comment "When applied to a file, this ACL entry grants the right to execute the file in-memory. When Applied to a Directory, grants Traversal rights into the Directory"@en ;
			rdfs:domain :ACLEntry ;
		    rdfs:range user:Group ,  user:UserAccount , :default .

:grantsReadTo 
			rdf:type owl:ObjectProperty ;
		    rdfs:label "grants reading by"@en ;
		    rdfs:comment "When applied to a file, this ACL entry grants the right to access the content of the file. When Applied to a Directory, grants content listing rights into the directory"@en ;
			rdfs:domain :ACLEntry ;
		    rdfs:range user:Group ,  user:UserAccount , :default .


:grantsWriteTo 
			rdf:type owl:ObjectProperty ;
		    rdfs:label "grants writing by"@en ;
		    rdfs:comment "When applied to a file, this ACL entry grants the right to modify the content of the file. When Applied to a Directory, grants new file or directory creation rights into the directory"@en ;
		    rdfs:domain :ACLEntry ;
		    rdfs:range user:Group ,  user:UserAccount , :default .


:hasACL
			rdf:type owl:ObjectProperty, owl:FunctionalProperty;
		    rdfs:label "has Access Control List"@en ;
		    rdfs:comment "this resource has an Access Control List governing account, group, role or location-specific access restrictions and capabilities."@en ;
		    owl:inverseOf :controlsAccessTo ;
		    rdfs:domain owl:Thing ;
		    rdfs:range :ACL .

:controlsAccessTo
			rdf:type owl:ObjectProperty ;
			rdfs:label "governs access to"@en ;
			rdfs:comment "This Access Control list contains the rules that grant (or deny) permissions to the listed resource, to the listed roles"@en ;
			rdfs:domain :ACL ;
			rdfs:range owl:Thing ;
			owl:inverseOf :hasACL .

:hasEntry
			rdf:type owl:InverseFunctionalProperty ,   owl:ObjectProperty ;
		    rdfs:label "has ACL entry"@en ;
		    rdfs:comment "the ACL has the following entry that defines access to a particular role"@en ; 
		    rdfs:subPropertyOf mere:hasPart ;
		    rdfs:domain :ACL ;
		    rdfs:range :ACLEntry ;
		    owl:inverseOf :isEntryIn .


:isEntryIn
			rdf:type owl:FunctionalProperty ,  owl:ObjectProperty ;          
			rdfs:label "is member of access control list"@en ;
			rdfs:comment "This Entry is part of an overall list of access control rules, often meaning that it will be assessed in order relative to other entries in the list."@en ;
		        rdfs:subPropertyOf mere:partOf ;
		    rdfs:domain :ACLEntry ;
		    rdfs:range :ACL ;
		    owl:inverseOf :hasEntryIn .

:isRecursive
			rdf:type owl:DatatypeProperty ,  owl:FunctionalProperty ;
		    rdfs:label "is recursive"@en ;
		    rdfs:comment "recursive ACL entries grant their permissions to all child objects of the listed object."@en ;
		    rdfs:domain :ACL ;
		    rdfs:range xsd:boolean .

:hasOrder
			rdf:type owl:DatatypeProperty ,  owl:FunctionalProperty ;
		    rdfs:label "is at position number"@en ;
		    rdfs:comment "The Access Control entry's position within the Access Control List"@en ;
		    rdfs:domain :ACLEntry ;
		    rdfs:range xsd:integer .

:ACL
			rdf:type owl:Class ;
		    rdfs:subClassOf owl:Thing ;
		    rdfs:subClassOf mere:Composite ;
	            rdfs:label "Access Control List"@en ;
		    rdfs:comment "A list of Access Control Entries, describing the rights to a resource to specific identities and identify groups."@en .

:ACLEntry
			rdf:type owl:Class ;
		    rdfs:subClassOf owl:Thing ;
		    rdfs:subClassOf mere:Atom ;
		    rdfs:label "ACL Entry"@en ;
		    rdfs:comment "Access Control Lists are lists of Access Control Entries. This is a single entry, usually specifying a particular account or role's access, to the resources governed by the Access Control List it is contained in."@en .
			
:FilesystemACL
			rdf:type owl:Class ;
			rdfs:label "File System Access Control List"@en ;
		    rdfs:subClassOf :ACL ;
		    rdfs:comment "An access control list specifying CRUDE rights to files and directories"@en .

:hasExecuteAccessTo rdf:type owl:ObjectProperty ;
                 rdfs:label "grants execution by"@en ;
                 rdfs:comment "When applied to a file, this ACL entry grants the right to execute the file in-memory. When Applied to a Directory, grants Traversal rights into the Directory"@en ;
				 owl:inverseOf :grantsExecuteTo ;
				 rdfs:range :ACLEntry ;
                 rdfs:domain user:Group ,  user:UserAccount , :default .


:hasReadAccessTo rdf:type owl:ObjectProperty ;
                 rdfs:label "grants execution by"@en ;
                 rdfs:comment "When applied to a file, this ACL entry grants the right to execute the file in-memory. When Applied to a Directory, grants Traversal rights into the Directory"@en ;
				 owl:inverseOf :grantsReadTo ;
				 rdfs:range :ACLEntry ;
                 rdfs:domain user:Group ,  user:UserAccount , :default .

:hasWriteAccessTo rdf:type owl:ObjectProperty ;
                 rdfs:label "grants execution by"@en ;
                 rdfs:comment "When applied to a file, this ACL entry grants the right to execute the file in-memory. When Applied to a Directory, grants Traversal rights into the Directory"@en ;
				 owl:inverseOf :grantsWriteTo ;
				 rdfs:range :ACLEntry ;
                 rdfs:domain user:Group ,  user:UserAccount , :default .

:NetworkACL
			rdf:type owl:Class ;
			rdfs:subClassOf :ACL ;
			rdfs:label "Network Access Control List"@en ;
		    rdfs:comment "An access control list specifying allowable connection types between network segments"@en .

:NtfsACL
			rdf:type owl:Class ;
		    rdfs:label "NTFS Filesystem ACL"@en ;
		    rdfs:comment "An access control list for an NTFS Filesystem"@en ;
		    rdfs:subClassOf :FilesystemACL .

:PosixACL
			rdf:type owl:Class ;
			rdfs:label "POSIX style Filesystem ACL"@en ;
			rdfs:comment "An access list in the owner-group-world POSIX standard style"@en ;
			rdfs:subClassOf :FilesystemACL .
		

:DefaultEntry
			rdf:type owl:Class ;
			rdfs:subClassOf :ACLEntry ;
			rdfs:label "Default Permissions Entry"@en ;
			rdfs:comment "The default permissions granted by this ACL to any entity not explicity listed"@en .

:hasDefault
			rdf:type owl:ObjectProperty , owl:FunctionalProperty ;
			rdfs:subPropertyOf :hasEntry ;
			rdfs:label "has Default Entry"@en ;
			rdfs:comment "The Default entry in an ACL when no other entry can be applied to the resource requester"@en ;
			rdfs:domain :ACL ;
			rdfs:range :DefaultEntry .
				
:isDefaultIn
			rdf:type owl:ObjectProperty , owl:FunctionalProperty;
			rdfs:subPropertyOf :isEntryIn ;
			rdfs:label "is Default Entry"@en ;
			rdfs:comment "The Default entry in an ACL when no other entry can be applied to the resource requester"@en ;
			rdfs:domain :ACL ;
			rdfs:range :DefaultEntry .

:default
			rdf:type owl:Class ;
			rdfs:subClassOf owl:Thing ;
			rdfs:label "An ACL Default"@en ;
			rdfs:comment "Used only to indicate that an ACL Entry represents default permissions issued globally" .

:Everyone
			rdf:type owl:NamedIndividual , :default;
			rdfs:label "Everyone" ;
			rdfs:comment "A Default Entry indicating global defaults" .
				
:AllUsers
			rdf:type owl:NamedIndividual , :default;
			rdfs:label "All Users" ;
			rdfs:comment "A Default Entry indicating global defaults" .

:AllGroups
			rdf:type owl:NamedIndividual , :default;
			rdfs:label "All Groups" ;
			rdfs:comment "A Default Entry indicating global defaults" .

