@prefix rdf: <http://www.w3.org/1999/02/22-rdf-syntax-ns#> .
@prefix rdfs: <http://www.w3.org/2000/01/rdf-schema#> .
@prefix xsd: <http://www.w3.org/2001/XMLSchema#> .
@prefix xml: <http://www.w3.org/XML/1998/namespace> .
@prefix dc: <http://purl.org/dc/elements/1.1/#> .
@prefix owl: <http://www.w3.org/2002/07/owl#> .
@prefix owl2: <http://www.w3.org/2006/12/owl2#> .
@prefix swrlx: <http://www.w3.org/2003/11/swrlx#> .
@prefix event: <http://purl.org/NET/c4dm/event.owl#> .
@prefix time: <http://www.w3.org/2006/time#> .
@prefix foaf: <http://xmlns.com/foaf/0.1/> .

@prefix tapio: <http://www.invincea.com/ontologies/icas/1.0/tapio#> .
@prefix user: <http://www.invincea.com/ontologies/icas/1.0/user#> .
@prefix host: <http://www.invincea.com/ontologies/icas/1.0/host#> .
@prefix process: <http://www.invincea.com/ontologies/icas/1.0/process#> .
@prefix ipnet: <http://www.invincea.com/ontologies/icas/1.0/ipnet#> .
@prefix : <http://www.invincea.com/ontologies/icas/1.0/authentication#> .
@base <http://www.invincea.com/ontologies/icas/1.0/authentication> .

<http://www.invincea.com/ontologies/icas/1.0/authentication>
			rdf:type owl:Ontology ;
			rdfs:label "Authentication Ontology"@en ;
			rdfs:comment "Describes elements related to authentication mechanisms in systems that grant identity to users and requests to map them to privileges"@en ;
			dc:description "Describes elements related to authentication mechanisms in systems that grant identity to users and requests to map them to privileges"@en ;
			owl:versionInfo "1.0" ;
			dc:creator: "Invincea Labs"@en ;
			dc:date "2014" ;
			owl:imports <http://www.invincea.com/ontologies/icas/1.0/host> ,
    					<http://www.invincea.com/ontologies/icas/1.0/user> .

			
:Credential 
			rdf:type owl:Class ;
			rdfs:subClassOf owl:Thing ;
			rdfs:label "Credential"@en ;
			rdfs:comment "A credential that can be used for authentication."@en .

:LoginCredential
			rdf:type owl:Class ;
			rdfs:subClassOf :Credential ;
			rdfs:label "Login Credential"@en ;
			rdfs:comment "The generic set of credentials which are authenticated using a username  and (optionally) a password."@en .

:AuthEvent
			rdf:type owl:Class ;
			rdfs:subClassOf event:Event ;
			rdfs:label "Authentication Event"@en ;
			rdfs:comment "A generic attempt by a user to authenticate to a service."@en .

:AuthProvider
			rdf:type owl:Class ;
			rdfs:subClassOf owl:Thing ;
			rdfs:label "Authentication Provider"@en ;
			rdfs:comment "A provider capable of providing authentication services. Examples might include RADIUS, local, etc."@en .

:authBy
			rdf:type owl:FunctionalProperty ,  owl:ObjectProperty ;
			rdfs:label "authenticated By"@en ;
			rdfs:comment "Relates an authentication provider to an authentication event. "@en ;
			rdfs:subPropertyOf event:agent ;
			rdfs:domain :AuthEvent ;
			rdfs:range :AuthProvider .

:authToHost
			rdf:type owl:FunctionalProperty ,  owl:ObjectProperty ;
			rdfs:label "authenticating To" ;
			rdfs:comment "The host that this authentication event is providing authentication for."@en ;
			rdfs:subPropertyOf event:factor ;
			rdfs:domain :AuthEvent ;
			rdfs:range host:Host .

:authRequestedFrom 
			rdf:type owl:FunctionalProperty ,  owl:ObjectProperty ;
			rdfs:label "authentication attempted from" ;
			rdfs:comment "The Source of the authentication attempt. The client endpoint of an authentication connection."@en ;
			rdfs:subPropertyOf event:factor ;
			rdfs:domain :AuthEvent ;
			rdfs:range host:Host , ipnet:Address .

:hasCredential
			rdf:type owl:ObjectProperty ;
			rdfs:label "has credential"@en ;
			rdfs:comment "Links user#UserAccount to credential sets."@en ;
			rdfs:domain user:UserAccount ;
			rdfs:range :Credential ;
			owl:equivalentProperty user:hasCredential .

:usingCredential
			rdf:type owl:FunctionalProperty ,  owl:ObjectProperty ;
			rdfs:label "Authenticated With Credential"@en ;
			rdfs:comment "The credential token presented to verify  that the user is who they attest to be during this authentication session"@en ;
			rdfs:subPropertyOf event:factor ;
			rdfs:range :Credential ;
			rdfs:domain :AuthEvent .

:authStatus
			rdf:type owl:DatatypeProperty ,  owl:FunctionalProperty ;
			rdfs:label "Authentication Status"@en ;
			rdfs:comment "The status of an authentication event. Could be 'success', 'failure', 'inprogress', etc."@en ;
			rdfs:domain :AuthEvent ;
			rdfs:range xsd:string .

:sessionId
            rdf:type owl:DatatypeProperty ,   owl:FunctionalProperty ;
			rdfs:label "Unique ID for the authentication session"@en ;            
			rdfs:comment "The unique session ID given to this authentication event."@en ;
			rdfs:domain :AuthEvent ;
			tapio:signaturePriority 1 ;
			rdfs:range xsd:string .            

:loginName
			rdf:type owl:DatatypeProperty ,  owl:FunctionalProperty ;
			rdfs:label "Login Name"@en ;
			rdfs:comment "The specific string used to identify an account via keyboard input"@en ;
			rdfs:domain :LoginCredential ;
			tapio:signaturePriority 2 ;
			rdfs:range xsd:string .

:loginPass 
			rdf:type owl:DatatypeProperty ,  owl:FunctionalProperty ;
			rdfs:label "Login Password"@en ;
			rdfs:comment "A password or passphrase used for login credentials"@en ;
			rdfs:domain :LoginCredential ;
			rdfs:range xsd:string .

:authenticatesAgainstRealm
			rdf:type owl:ObjectProperty ,  owl:FunctionalProperty ;
			rdfs:label "authenticates against account realm"@en ;
			rdfs:domain :AuthProvider ;
			rdfs:range user:Realm .

:LocalAccount
			rdf:type :AuthProvider ,  owl:NamedIndividual ;
			rdfs:label "Local Host Account Authenticator"@en;
			rdfs:comment "A local host account, such as controlled by PAM or Windows Account Services."@en .

:RADIUS
			rdf:type :AuthProvider ,   owl:NamedIndividual ;
			rdfs:label "RADIUS Authenticator"@en ;
			rdfs:comment "A RADIUS remote authentication service." .

:LDAP
			rdf:type :AuthProvider ,   owl:NamedIndividual ;
			rdfs:label "LDAP Authenticator"@en ;
			rdfs:comment "An LDAP authentication service." .

:ActiveDirectory
			rdf:type :AuthProvider ,   owl:NamedIndividual ;
			rdfs:label "LDAP Service"@en ;
			rdfs:comment "An ActiveDirectory authentication service." .
