@prefix rdf: <http://www.w3.org/1999/02/22-rdf-syntax-ns#> .
@prefix rdfs: <http://www.w3.org/2000/01/rdf-schema#> .
@prefix xsd: <http://www.w3.org/2001/XMLSchema#> .
@prefix xml: <http://www.w3.org/XML/1998/namespace> .
@prefix dc: <http://purl.org/dc/elements/1.1/#> .
@prefix owl: <http://www.w3.org/2002/07/owl#> .
@prefix owl2: <http://www.w3.org/2006/12/owl2#> .
@prefix swrlx: <http://www.w3.org/2003/11/swrlx#> .
@prefix event: <http://purl.org/NET/c4dm/event.owl#> .
@prefix time: <http://www.w3.org/2006/time#> .
@prefix foaf: <http://xmlns.com/foaf/0.1/> .

@prefix mere: <http://www.bbn.com/ontologies/domain/foundation/mereology#> .
@prefix nic: <http://www.invincea.com/ontologies/icas/1.0/nic#> .
@prefix tapio: <http://www.invincea.com/ontologies/icas/1.0/tapio#> .
@prefix ipnet: <http://www.invincea.com/ontologies/icas/1.0/ipnet#> .
@prefix host: <http://www.invincea.com/ontologies/icas/1.0/host#> .
@prefix : <http://www.invincea.com/ontologies/icas/1.0/dhcp#> .
@base <http://www.invincea.com/ontologies/icas/1.0/dhcp> .

<http://www.invincea.com/ontologies/icas/1.0/dhcp> 
			rdf:type owl:Ontology ;
			rdfs:label "Dynamic Host Control Protocol Ontology"@en ;
			rdfs:comment "an ontology of DHCP Leases and Services."@en ;
			dc:description "Describes elements related to authentication mechanisms in systems that grant identity to users and requests to map them to privileges"@en ;
			owl:versionInfo "1.0" ;
			dc:creator "Invincea Labs"@en ;
			dc:date "2014" ;
			owl:imports <http://www.invincea.com/ontologies/icas/1.0/user> ,
    					<http://www.invincea.com/ontologies/icas/1.0/ipnet> .


:Pool 
			rdf:type owl:Class ;
			rdfs:label "DHCP IP Address Pool"@en ;
			rdfs:comment "DHCP assigns addresses to systems from a pool of assigned addresses. "@en ;
			rdfs:subClassOf owl:Thing ;
			rdfs:subClassOf mere:Composite .

:inPool 
			rdf:type owl:ObjectProperty ;
			rdfs:label "belongs to DHCP Pool"@en ;
			rdfs:comment "this address has been allocated to a DHCP Pool, and is not permanently assigned to any particular host"@en ;
			rdfs:subPropertyOf mere:partOf ;
			rdfs:domain ipnet:Address ;
			rdfs:range :Pool ;
			owl:inverseOf :containsAddress .

:containsAddress 
			rdf:type owl:InverseFunctionalProperty ,  owl:ObjectProperty ;
			rdfs:label "controls assignment of"@en ;
			rdfs:comment "this DHCP address pool is authoritative for this IP address, and controls leasing of it to client systems."@en ;
			rdfs:subPropertyOf mere:hasPart ;
			rdfs:domain :Pool ;
			rdfs:range ipnet:Address ;
			tapio:signaturePriority 1 ;
			owl:inverseOf :inPool .

:Lease 
			rdf:type owl:Class ;
			rdfs:label "DHCP Lease"@en ;
			rdfs:comment "A Lease for a single IP Address from a DHCP Pool to a Network Interface on a Host"@en;
			rdfs:subClassOf owl:Thing .

:leased 
			rdf:type owl:ObjectProperty ;
			rdfs:label "was granted lease"@en ;
			rdfs:comment "this NIC was successfully granted this DHC lease for an IP Address"@en ;
			rdfs:domain nic:NIC ;
			rdfs:range :Lease ;
			owl:inverseOf :leasedTo .

:leasedto 
			rdf:type owl:FunctionalProperty ,   owl:ObjectProperty ;
			rdfs:label "was issued to"@en ;
			rdfs:comment "this lease was succesfully issued to a requesting NIC to grant it a temporary IP Address"@en ;
			rdfs:domain :Lease ;
			rdfs:range nic:NIC ;
			owl:inverseOf :leased .

:leaseEnd
			rdf:type owl:DatatypeProperty ,   owl:FunctionalProperty ;
			rdfs:label "lease ended on"@en ;
			rdfs:comment "when the lease expired"@en ;
			rdfs:domain :Lease ;
			rdfs:range xsd:dateTimeStamp .

:leaseStart
			rdf:type owl:DatatypeProperty,   owl:FunctionalProperty ;
			rdfs:label "lease ended on"@en ;
			rdfs:comment "when the lease was granted"@en ;
			rdfs:domain :Lease ;
			rdfs:range xsd:dateTimeStamp .

:forAddress
			rdf:type owl:FunctionalProperty ,  owl:ObjectProperty ;
			rdfs:label "for address"@en ;
			rdfs:comment "the IP Address that was granted via a successful DHCP Lease"@en ;
			rdfs:domain :Lease ;
			rdfs:range ipnet:Address .

:forHostName
			rdf:type owl:ObjectProperty ;
			rdfs:label "for hostname"@en ;
			rdfs:comment "leases may identify themselves with a particular hostname, which may have its associated DNS Entry updated once the lease is granted. This is used extensively in Microsoft Active Directory"@en ;
			rdfs:domain host:Host ;
			rdfs:range :Lease .

:fromAuthority
			rdf:type owl:FunctionalProperty ,   owl:ObjectProperty ;
			rdfs:label "issued from"@en ;
			rdfs:comment "the NIC (and therefore MAC) address this lease was issued by."@en ;
			rdfs:domain :Lease ;
			rdfs:range nic:NIC ;
			owl:inverseOf :issuedLease .

:issuedLease	
			rdf:type owl:ObjectProperty ;
			rdfs:label "issued lease"@en ;
			rdfs:comment "This NIC issued a DHCP to the requesting NIC"@en ;
			rdfs:range :Lease ;
			rdfs:domain nic:NIC ;
			owl:inverseOf :fromAuthority .
