@prefix rdf: <http://www.w3.org/1999/02/22-rdf-syntax-ns#> .
@prefix rdfs: <http://www.w3.org/2000/01/rdf-schema#> .
@prefix xsd: <http://www.w3.org/2001/XMLSchema#> .
@prefix xml: <http://www.w3.org/XML/1998/namespace> .
@prefix dc: <http://purl.org/dc/elements/1.1/#> .
@prefix owl: <http://www.w3.org/2002/07/owl#> .
@prefix owl2: <http://www.w3.org/2006/12/owl2#> .
@prefix swrlx: <http://www.w3.org/2003/11/swrlx#> .
@prefix event: <http://purl.org/NET/c4dm/event.owl#> .
@prefix time: <http://www.w3.org/2006/time#> .
@prefix foaf: <http://xmlns.com/foaf/0.1/> .

@prefix nic: <http://www.invincea.com/ontologies/icas/1.0/nic#> .
@prefix oui: <http://www.invincea.com/ontologies/icas/1.0/oui#> .
@prefix user: <http://www.invincea.com/ontologies/icas/1.0/user#> .
@prefix filesystem: <http://www.invincea.com/ontologies/icas/1.0/filesystem#> .
@prefix tapio: <http://www.invincea.com/ontologies/icas/1.0/tapio#> .
@prefix ipnet: <http://www.invincea.com/ontologies/icas/1.0/ipnet#> .
@prefix hardware: <http://www.invincea.com/ontologies/icas/1.0/hardware#> .
@prefix process: <http://www.invincea.com/ontologies/icas/1.0/process#> .
@prefix osplatform: <http://www.invincea.com/ontologies/icas/1.0/osplatform#> .
@prefix : <http://www.invincea.com/ontologies/icas/1.0/host#> .
@base <http://www.invincea.com/ontologies/icas/1.0/host> .

<http://www.invincea.com/ontologies/icas/1.0/host> 
			rdf:type owl:Ontology ;
			rdfs:label "Computing Host Ontology"@en ;
			rdfs:comment "Describes discrete computing Hosts"@en ;
			dc:description "Describes discrete computing Hosts"@en ;
    		owl:versionInfo "1.0" ;
    		dc:creator: "Invincea Labs"@en ;
    		dc:date "2014" ;
			owl:imports <http://www.invincea.com/ontologies/icas/1.0/hardware> ,
						<http://www.invincea.com/ontologies/icas/1.0/nic> ,
						<http://www.invincea.com/ontologies/icas/1.0/osplatform> ,
						<http://www.invincea.com/ontologies/icas/1.0/user> .

			
:UsedByUser 
			rdf:type owl:ObjectProperty ;
			rdfs:label "is used by"@en ;
			rdfs:comment "authenticated activity from this user has been observed on this host."@en ;
			rdfs:domain :Host ;
			rdfs:range user:UserAccount .

:existsAs 
			rdf:type owl:FunctionalProperty ,  owl:ObjectProperty ;
			rdfs:label "exists as device"@en ;
			rdfs:comment "the physical or virtual hardware underlying the operating system of this host"@en ;
			rdfs:range hardware:ComputingMachine ;
			rdfs:domain :Host .

:hasAgent 
			rdf:type owl:FunctionalProperty ,  owl:ObjectProperty ;
			rdfs:label "has TAPIO Agent"@en ;
			rdfs:domain :Host ;
			tapio:signaturePriority 1 ; 
			rdfs:range tapio:Agent .

:hasFileSystemRoot 
			rdf:type owl:InverseFunctionalProperty ,  owl:ObjectProperty ;
			rdfs:label "has a filesystem root at"@en ;
			rdfs:comment "a root (top-level) Directory from while the system may access file resources by names relative to"@en ;
			owl:inverseOf filesystem:isFilesystemRootOn ;
			rdfs:domain :Host ;
			rdfs:range filesystem:Directory .

:hasNIC 
			rdf:type owl:InverseFunctionalProperty ,  owl:ObjectProperty ;
			rdfs:label "has network interface"@en ;
			rdfs:comment "this host is bonded to a network interface. Hosts may have many network interfaces, and many hosts may utilize a NIC in some abstracted way, but only a single host can have direct (driver-level control) of the device."@en ;
			rdfs:domain :Host ;
			rdfs:range nic:NIC .

:hasProcessList 
			rdf:type owl:FunctionalProperty ,   owl:ObjectProperty ;
			rdfs:label "has Process List"@en ;
			rdfs:domain :Host ;
			rdfs:range process:ProcessList ;
			owl:inverseOf process:onHost .

:hostName 
			rdf:type owl:DatatypeProperty ,   owl:FunctionalProperty ;
			rdfs:label "has host name"@en ;
			rdfs:comment "the internal hostname this system refers to itself as. May differ from other name-based systems (such as DNS)."@en ;
			rdfs:domain :Host ;
			tapio:signaturePriority 4 ; 
			rdfs:range xsd:string .
                    
:Host
			rdf:type owl:Class ;
			rdfs:label "Host"@en ;
			rdfs:comment "A single host, as an abstract concept. Hosts are the intersection between hardware (physical or virtual), an instance of an operating system and associated software.  Can also be though of as a code execution compartment - a kernel with associated single process table."@en .

:IPenabledDevice 
			rdf:type owl:Class ;
			rdfs:label "IP Enabled Device"@en ;
			rdfs:comment "A TCP/IP Connected Device that does not fall into the idea of a general computing machine"@en ;                
			rdfs:subClassOf :Host .

:Infrastructure 
			rdf:type owl:Class ;
			rdfs:label "Infrastructure Host"@en ;
			rdfs:comment "A Host that is a critical piece of the surrounding infrastructure - typically a router, switch or other connectivity device"@en ;                   
			rdfs:subClassOf :Host .

:Mobile 
			rdf:type owl:Class ;
			rdfs:label "Mobile Host"@en ;
			rdfs:comment "A Physically mobile device that is expected to move from network to networ with some regularity"@en ;  
			rdfs:subClassOf :Host .

:Server 
			rdf:type owl:Class ;
			rdfs:label "Server Host"@en ;
			rdfs:comment "A Host that is expected to be at a predictable location or address, providing network services to a number of client hosts"@en ; 
			rdfs:subClassOf :Host .

:Workstation 
			rdf:type owl:Class ;
			rdfs:label "Workstation Host"@en ;
			rdfs:subClassOf :Host ;
			rdfs:comment "A machine intended to be used locally, by a single primary user, from a fixed location and network"@en .
