@prefix rdf: <http://www.w3.org/1999/02/22-rdf-syntax-ns#> .
@prefix rdfs: <http://www.w3.org/2000/01/rdf-schema#> .
@prefix xsd: <http://www.w3.org/2001/XMLSchema#> .
@prefix xml: <http://www.w3.org/XML/1998/namespace> .
@prefix dc: <http://purl.org/dc/elements/1.1/#> .
@prefix owl: <http://www.w3.org/2002/07/owl#> .
@prefix owl2: <http://www.w3.org/2006/12/owl2#> .
@prefix swrlx: <http://www.w3.org/2003/11/swrlx#> .
@prefix event: <http://purl.org/NET/c4dm/event.owl#> .
@prefix time: <http://www.w3.org/2006/time#> .
@prefix foaf: <http://xmlns.com/foaf/0.1/> .

@prefix : <http://www.invincea.com/ontologies/icas/1.0/host-inferred#> .
@prefix tapio: <http://www.invincea.com/ontologies/icas/1.0/tapio#> .
@prefix process: <http://www.invincea.com/ontologies/icas/1.0/process#> .
@prefix host: <http://www.invincea.com/ontologies/icas/1.0/host#> .
@base <http://www.invincea.com/ontologies/icas/1.0/host-inferred> .

<http://www.invincea.com/ontologies/icas/1.0/host-inferred> 
			rdf:type owl:Ontology ;
			rdfs:label "Host Ontology - Inferred Axioms"@en ;
			owl:versionInfo "1.0"@en ;
			rdfs:comment "This ontology contains additional predicates to the Host ontology, intended to be computationally inferred via an OWL reasoner"@en ;
			owl:imports <http://www.invincea.com/ontologies/icas/1.0/host-applied> .


:ExposedHost 
			rdf:type owl:Class ;
			rdfs:label "Exposed Host"@en ;
			rdfs:subClassOf host:Host ;
			rdfs:comment "This host is directly exposed to attack, through a quantified exposure window"@en .

:PossiblyCompromisedHost 
			rdf:type owl:Class ;
			rdfs:label "Possibly Compromised Host"@en ;
			rdfs:subClassOf host:Host ;
			rdfs:comment "The relationships exhibited by this host and other elements connecting to it, indicate that there is a high probability the host is under the control of a hostile party."@en .

:VulnerableHost 
			rdf:type owl:Class ;
			rdfs:label "Vulnerable Host"@en ;
			rdfs:subClassOf host:Host ;
			rdfs:comment "This host is known to contain presently-known software vulnerabilities ccapable of granting a hostile party access to the system"@en .
