@prefix rdf: <http://www.w3.org/1999/02/22-rdf-syntax-ns#> .
@prefix rdfs: <http://www.w3.org/2000/01/rdf-schema#> .
@prefix xsd: <http://www.w3.org/2001/XMLSchema#> .
@prefix xml: <http://www.w3.org/XML/1998/namespace> .
@prefix dc: <http://purl.org/dc/elements/1.1/#> .
@prefix owl: <http://www.w3.org/2002/07/owl#> .
@prefix owl2: <http://www.w3.org/2006/12/owl2#> .
@prefix swrlx: <http://www.w3.org/2003/11/swrlx#> .
@prefix event: <http://purl.org/NET/c4dm/event.owl#> .
@prefix time: <http://www.w3.org/2006/time#> .
@prefix foaf: <http://xmlns.com/foaf/0.1/> .
@prefix mere: <http://www.bbn.com/ontologies/domain/foundation/mereology#> .
@prefix nic: <http://www.invincea.com/ontologies/icas/1.0/nic#> .
@prefix oui: <http://www.invincea.com/ontologies/icas/1.0/oui#> .
@prefix log: <http://www.invincea.com/ontologies/icas/1.0/log#> .
@prefix user: <http://www.invincea.com/ontologies/icas/1.0/user#> .
@prefix filesystem: <http://www.invincea.com/ontologies/icas/1.0/filesystem#> .
@prefix tapio: <http://www.invincea.com/ontologies/icas/1.0/tapio#> .
@prefix ipnet: <http://www.invincea.com/ontologies/icas/1.0/ipnet#> .
@prefix hardware: <http://www.invincea.com/ontologies/icas/1.0/hardware#> .
@prefix mime: <http://www.invincea.com/ontologies/icas/1.0/mime#> .
@prefix process: <http://www.invincea.com/ontologies/icas/1.0/process#> .
@prefix host: <http://www.invincea.com/ontologies/icas/1.0/host#> .
@prefix : <http://www.invincea.com/ontologies/icas/1.0/memory#> .
@base <http://www.invincea.com/ontologies/icas/1.0/memory> .

<http://www.invincea.com/ontologies/icas/1.0/memory> 
			rdf:type owl:Ontology ;
			rdfs:label "An ontology for mapping regions of Memory Objects into their functional purposes."@en ;
			rdfs:comment "Describes high level organization and addressing of objects within Random Access Memory"@en ;
			dc:description "Describes high level organization and addressing of objects within Random Access Memory"@en ;
    		owl:versionInfo "1.0" ;
    		dc:creator: "Invincea Labs"@en ;
    		dc:date "2014" ;
			owl:imports <http://www.invincea.com/ontologies/icas/1.0/filesystem> ,
						<http://www.invincea.com/ontologies/icas/1.0/process> .

			
:MemoryBlock 
			rdf:type owl:Class ;
			rdfs:subClassOf owl:Thing ;
			rdfs:subClassOf mere:Composite ;
			rdfs:label "Region of Memory"@en ;
			rdfs:comment "An area of system memory, contiguous between a start and end address"@en .

:Code rdf:type 
			owl:Class ;
			rdfs:label "Region of Memory"@en ;
			rdfs:comment "An area of system memory assigned for executable code"@en ;
			rdfs:subClassOf :MemoryBlock .

:Data rdf:type 
			owl:Class ;
			rdfs:label "Data Region of Memory"@en ;
			rdfs:comment "An area of system memory assigned for non-executable data"@en ;
			rdfs:subClassOf :MemoryBlock .

:MetaCode 
			rdf:type owl:Class ;
			rdfs:label "MetaCode Region of Memory"@en ;
			rdfs:comment "An area of system memory assigned for execution-tracking items, such as the Heap and Stack"@en ;
			rdfs:subClassOf :Code .

:MetaData 
			rdf:type owl:Class ;
			rdfs:label "MetaData Region of Memory"@en ;
			rdfs:comment "An area of system memory assigned for data-tracking items, such as item index pointers"@en ;
			rdfs:subClassOf :Data .
					
:MemoryAddressPhy64 
			rdf:type rdfs:Datatype ;
			rdfs:label "64-Bit Physical Memory Address"@en ;
			rdfs:comment "A 64bit address, relative to the host system's entire memory space"@en ;
			owl:equivalentClass xsd:unsignedInt .

:MemoryAddressPhy32 
			rdf:type rdfs:Datatype ;
			rdfs:label "32-Bit Physical Memory Address"@en ;
			rdfs:comment "A 32bit address, relative to the host system's entire memory space"@en ;
			owl:equivalentClass xsd:unsignedInt .
             		
:MemoryAddressVirt64 
			rdf:type rdfs:Datatype ;
			rdfs:label "64-Bit Virtual Memory Address"@en ;
			rdfs:comment "A 64bit address, relative to the host system's entire memory space"@en ;
			owl:equivalentClass xsd:unsignedLong .

:MemoryAddressVirt32 
			rdf:type rdfs:Datatype ;
			rdfs:label "32-Bit Virtual Memory Address"@en ;
			rdfs:comment "A 32bit address, relative to the host system's entire memory space"@en ;
			owl:equivalentClass xsd:unsignedInt .

:hasMemoryBlock 
			rdf:type owl:ObjectProperty ;
			rdfs:label "contains memory region"@en ;
			rdfs:comment "This process owns the identified block of memory"@en ; 
			rdfs:domain process:Process ;
			rdfs:range :MemoryBlock ;
			owl:inverseOf :isOwnedByProcess .

:isOwnedByProcess 
			rdf:type owl:FunctionalProperty , owl:ObjectProperty ;
			rdfs:label "is owned by process"@en ;
			rdfs:comment "the executing process that owns this region of memory"@en ;
			owl:inverseOf :hasMemoryBlock ;
			rdfs:domain :MemoryBlock ;
			rdfs:range process:Process .

:mappedFromFile 
			rdf:type owl:FunctionalProperty ,  owl:ObjectProperty ;
			rdfs:label "is loaded from contents of file"@en ;
			rdfs:comment "the contents of this memory block were drawn from this file."@en ;
			rdfs:range filesystem:File ;
			rdfs:domain :MemoryBlock .

:sharesVirtualMemorySpace 
			rdf:type owl:ObjectProperty , owl:SymmetricProperty ;
			rdfs:label "shares virtual memory space with"@en ;
			rdfs:domain :MemoryBlock ;
			rdfs:range :MemoryBlock .

:beginsAtAddress 
			rdf:type owl:DatatypeProperty ,  owl:FunctionalProperty ;
			rdfs:label "Begins at Address"@en ;
			tapio:signaturePriority 1 ; 
			rdfs:range :MemoryAddressPhy32, :MemoryAddressPhy64, :MemoryAddressVirt32, :MemoryAddressVirt64 ;
			rdfs:domain :MemoryBlock .

:endsAtAddress 
			rdf:type owl:DatatypeProperty ,  owl:FunctionalProperty ;
			rdfs:label "Ends at Address"@en ;
			tapio:signaturePriority 2 ; 
			rdfs:range :MemoryAddressPhy32, :MemoryAddressPhy64, :MemoryAddressVirt32, :MemoryAddressVirt64 ;
			rdfs:domain :MemoryBlock .

:hasSize 
			rdf:type owl:DatatypeProperty ,  owl:FunctionalProperty ;
			rdfs:label "Has total size"@en ;
			rdfs:domain :MemoryBlock ;
			rdfs:range xsd:positiveInteger .
