@prefix rdf: <http://www.w3.org/1999/02/22-rdf-syntax-ns#> .
@prefix rdfs: <http://www.w3.org/2000/01/rdf-schema#> .
@prefix xsd: <http://www.w3.org/2001/XMLSchema#> .
@prefix xml: <http://www.w3.org/XML/1998/namespace> .
@prefix dc: <http://purl.org/dc/elements/1.1/#> .
@prefix owl: <http://www.w3.org/2002/07/owl#> .
@prefix owl2: <http://www.w3.org/2006/12/owl2#> .
@prefix swrlx: <http://www.w3.org/2003/11/swrlx#> .
@prefix event: <http://purl.org/NET/c4dm/event.owl#> .
@prefix time: <http://www.w3.org/2006/time#> .
@prefix foaf: <http://xmlns.com/foaf/0.1/> .

@prefix tapio: <http://www.invincea.com/ontologies/icas/1.0/tapio#> .
@prefix oui: <http://www.invincea.com/ontologies/icas/1.0/oui#> .
@prefix hardware: <http://www.invincea.com/ontologies/icas/1.0/hardware#> .
@prefix ipnet: <http://www.invincea.com/ontologies/icas/1.0/ipnet#> .
@prefix host: <http://www.invincea.com/ontologies/icas/1.0/host#> .
@prefix : <http://www.invincea.com/ontologies/icas/1.0/nic#> .
@base <http://www.invincea.com/ontologies/icas/1.0/nic> .

<http://www.invincea.com/ontologies/icas/1.0/nic> 
			rdf:type owl:Ontology ;
			rdfs:label "Network Interface Card Ontology"@en ;
			rdfs:comment "Describes network interface adapters and other virtual layer-2 adapters"@en ;
			dc:description "Describes network interface adapters and other virtual layer-2 adapters"@en ;
			owl:versionInfo "1.0" ;
			dc:creator: "Invincea Labs"@en ;
			dc:date "2014" ;                          
			owl:imports <http://www.invincea.com/ontologies/icas/1.0/hardware> ,
						<http://www.invincea.com/ontologies/icas/1.0/host> ,
						<http://www.invincea.com/ontologies/icas/1.0/ipnet> ,
						<http://www.invincea.com/ontologies/icas/1.0/oui> .
			
:NIC 
			rdf:type owl:Class ;
			rdfs:label "Network Interface Card"@en ;
			rdfs:comment "A Device, created either in hardware or software, that allows an operating system to communicate with other hosts"@en .

:Ethernet 
			rdf:type owl:Class ;
			rdfs:label "Ethernet"@en ;
			rdfs:comment "Ethernet interfaces provide single-circuit-multiple-access frame-based communication between local area hosts"@en ;			
			rdfs:subClassOf :NIC .

:802_11 
			rdf:type owl:Class ;
			rdfs:label "Wireless Ethernet Interface"@en ;
			rdfs:comment "802.11 describes local area network interfaces that communicate via packet radio"@en ;
			rdfs:subClassOf :Ethernet .

:802_3 
			rdf:type owl:Class ;
			rdfs:label "Wired Ethernet Interface"@en ;
			rdfs:comment "802.3 describes local area network interfaces that communicate via 4-wire cable"@en ;			
			rdfs:subClassOf :Ethernet .

:FDDI 
			rdf:type owl:Class ;
			rdfs:label "Fiber Distrbuted Data Interface"@en ;
			rdfs:comment "FDDI is a dual-ring system over optical cables, often used for interconnect between networking devices"@en ;
			rdfs:subClassOf :NIC .

:FrameRelay 
			rdf:type owl:Class ;
			rdfs:label "Frame Relay CSU/DSU"@en ;
			rdfs:comment "Frame Relay is a common wide area network interface, supporting multiple virtual circuits over the same line"@en ;
			rdfs:subClassOf :NIC .

:ATM
			rdf:type owl:Class ;
			rdfs:label "Asynchronous Transfer Mode"@en ;
			rdfs:comment "Asynchronous Transfer Mode Interfaces implement "@en ;
			rdfs:subClassOf :NIC .

:L2TP 
			rdf:type owl:Class ;
			rdfs:label "Layer 2 Tunnelling Protocol Interface"@en ;
			rdfs:comment "Layer 2 Tunnel Protocol is a software-defined network interface used to create virtal network topologies over existing physical networks"@en ;
			rdfs:subClassOf :PTP .

:PTP 
			rdf:type owl:Class ;
			rdfs:label "Point-To-Point Interface"@en ;
			rdfs:comment "Point-To-Point interfaces are software or hardware interfaces that only connect exactly two systems directly to one another"@en ;
			rdfs:subClassOf :NIC .

:SONET 
			rdf:type owl:Class ;
			rdfs:label "Synchronous Optical Networking Interface"@en ;
			rdfs:comment "SONET is a combined voice and data interface using optical cables, commonly used in backbone trunking"@en ;
			rdfs:subClassOf :NIC .

:hasIPaddress 
			rdf:type owl:InverseFunctionalProperty ,   owl:ObjectProperty ;
			rdfs:label "has IP Address"@en ;
			rdfs:comment "An IP Address must be attached to a network adapter (whether physical or virtual) to enable communication via that address. Pairings of addresses to Interfaces must be unique within a network."@en ;
			rdfs:range ipnet:Address ;
			rdfs:domain :NIC .

:hasNIC 
			rdf:type owl:InverseFunctionalProperty ,  owl:ObjectProperty ;
			rdfs:label "has Network Interface"@en ;
			rdfs:comment "this host has the following network interface available"@en ;
			rdfs:range :NIC ;
			rdfs:domain host:Host ;
			owl:inverseOf :onHost .

:hasOUI 
			rdf:type owl:FunctionalProperty ,  owl:ObjectProperty ;
			rdfs:label "manufactured by"@en ;
			rdfs:comment "the first portion of a MAC address is a unique sequence assigned to a particular manufacturer, to prevent MAC address collisions between network cards created by different companies."@en ;
			rdfs:domain :NIC ;
			rdfs:range oui:OUI .

:isHardware 
			rdf:type owl:FunctionalProperty ,  owl:ObjectProperty ;
			rdfs:label "exists as hardware device"@en ;
			rdfs:comment "the physical electronics that implement this network interface."@en ;
			rdfs:range hardware:Communications ;
			rdfs:domain :NIC .

:onHost 
			rdf:type owl:FunctionalProperty ,   owl:ObjectProperty ;
			rdfs:label "on Host"@en ;
			rdfs:comment "the Host this Network card connects to."@en ;
			rdfs:domain :NIC ;
			tapio:signaturePriority 1 ; 
			rdfs:range host:Host ;
			owl:inverseOf :hasNIC .

:hasMAC 
			rdf:type owl:DatatypeProperty ,  owl:FunctionalProperty ;
			rdfs:label "has MAC address"@en ;
			rdfs:comment "this interface is uniquely identified by the following 48-bit Media Access Control Address"@en ;			
			rdfs:domain :Ethernet ;
			tapio:signaturePriority 2 ; 
			rdfs:range :MAC .

:inBytes 
			rdf:type owl:DatatypeProperty ,  owl:FunctionalProperty ;
			rdfs:label "Received Bytes"@en ;
			rdfs:comment "The number of bytes successfully recieved by this interface since it was brought online"@en ;			
			rdfs:domain :NIC ;
			rdfs:range xsd:unsignedLong .

:inDrops 
			rdf:type owl:DatatypeProperty ,   owl:FunctionalProperty ;
			rdfs:label "Inbound Dropped Packets"@en ;
			rdfs:comment "The number of bytes unsuccessfully recieved by this interface since it was brought online"@en ;			
			rdfs:domain :NIC ;
			rdfs:range xsd:unsignedLong .

:inErrors 
			rdf:type owl:DatatypeProperty , owl:FunctionalProperty ;
			rdfs:label "Inbound Errors"@en ;
			rdfs:comment "The number of errors reported while recieving data by this interface since it was brought online"@en ;			
			rdfs:domain :NIC ;
			rdfs:range xsd:unsignedLong .

:inPackets 
			rdf:type owl:DatatypeProperty ,  owl:FunctionalProperty ;
			rdfs:label "Recieved Packets"@en ;
			rdfs:comment "The number of network packets recieved by this interface since it was brought online"@en ;
			rdfs:domain :NIC ;
			rdfs:range xsd:unsignedLong .

:outBytes 
			rdf:type owl:DatatypeProperty ,  owl:FunctionalProperty ;
			rdfs:label "Transmitted Bytes"@en ;
			rdfs:comment "The number of bytes successfully transmitted by this interface since it was brought online"@en ;			
			rdfs:domain :NIC ;
			rdfs:range xsd:unsignedLong .

:outDrops 
			rdf:type owl:DatatypeProperty ,   owl:FunctionalProperty ;
			rdfs:label "Outbound Dropped Packets"@en ;
			rdfs:comment "The number of network packets unsuccessfully transmitted by this interface since it was brought online"@en ;			
			rdfs:domain :NIC ;
			rdfs:range xsd:unsignedLong .

:outErrors 
			rdf:type owl:DatatypeProperty ,   owl:FunctionalProperty ;
			rdfs:label "Outbound Errors"@en ;
			rdfs:comment "The number of errors reported while recieving data by this interface since it was brought online"@en ;			
			rdfs:domain :NIC ;
			rdfs:range xsd:unsignedLong .

:outPackets 
			rdf:type owl:DatatypeProperty ,  owl:FunctionalProperty ;
			rdfs:label "Outbound Packets"@en ;
			rdfs:comment "The number of network packets successfully transmitted by this interface since it was brought online"@en ;
			rdfs:domain :NIC ;
			rdfs:range xsd:unsignedLong .

:MAC 
			rdf:type rdfs:Datatype ;
			rdfs:label "Media Access Control Address"@en ;
			rdfs:comment "The standard 48-bit hexadecimal address scheme used to assign a globally unique identifier to network interfaces"@en .

