@prefix rdf: <http://www.w3.org/1999/02/22-rdf-syntax-ns#> .
@prefix rdfs: <http://www.w3.org/2000/01/rdf-schema#> .
@prefix xsd: <http://www.w3.org/2001/XMLSchema#> .
@prefix xml: <http://www.w3.org/XML/1998/namespace> .
@prefix dc: <http://purl.org/dc/elements/1.1/#> .
@prefix owl: <http://www.w3.org/2002/07/owl#> .
@prefix owl2: <http://www.w3.org/2006/12/owl2#> .
@prefix swrlx: <http://www.w3.org/2003/11/swrlx#> .
@prefix event: <http://purl.org/NET/c4dm/event.owl#> .
@prefix time: <http://www.w3.org/2006/time#> .
@prefix foaf: <http://xmlns.com/foaf/0.1/> .
@prefix mere: <http://www.bbn.com/ontologies/domain/foundation/mereology#> .
@prefix tapio: <http://www.invincea.com/ontologies/icas/1.0/tapio#> .
@prefix nic: <http://www.invincea.com/ontologies/icas/1.0/nic#> .
@prefix oui: <http://www.invincea.com/ontologies/icas/1.0/oui#> .
@prefix log: <http://www.invincea.com/ontologies/icas/1.0/log#> .
@prefix user: <http://www.invincea.com/ontologies/icas/1.0/user#> .
@prefix filesystem: <http://www.invincea.com/ontologies/icas/1.0/filesystem#> .
@prefix ipnet: <http://www.invincea.com/ontologies/icas/1.0/ipnet#> .
@prefix authentication: <http://www.invincea.com/ontologies/icas/1.0/authentication#> .
@prefix hardware: <http://www.invincea.com/ontologies/icas/1.0/hardware#> .
@prefix mime: <http://www.invincea.com/ontologies/icas/1.0/mime#> .
@prefix host: <http://www.invincea.com/ontologies/icas/1.0/host#> .
@prefix : <http://www.invincea.com/ontologies/icas/1.0/process#> .
@base <http://www.invincea.com/ontologies/icas/1.0/process> .

<http://www.invincea.com/ontologies/icas/1.0/process> 
			rdf:type owl:Ontology ;
			rdfs:label "Process Execution Ontology"@en ;
			rdfs:comment "Describes the general organizational structure of executing processes in an operating system. It principally presents processes from an end-user/userspace viewpoint, using the same information available in normal management tools."@en ;
    		dc:description "Describes the general organizational structure of executing processes in an operating system. It principally presents processes from an end-user/userspace viewpoint, using the same information available in normal management tools."@en ;
			owl:versionInfo "1.0" ;
			dc:creator: "Invincea Labs"@en ;
			dc:date "2014" ;
			owl:imports <http://www.invincea.com/ontologies/icas/1.0/filesystem> ,
						<http://www.invincea.com/ontologies/icas/1.0/host> ,
						<http://www.invincea.com/ontologies/icas/1.0/ipnet> ,
						<http://www.invincea.com/ontologies/icas/1.0/log> ,
						<http://www.invincea.com/ontologies/icas/1.0/user> .

:socketState 
			rdf:type rdfs:Datatype , owl:FunctionalProperty ;
			rdfs:label "Socket State"@en ;
			rdfs:comment "The current state flag of a Socket, indicating the general behavior of the socket (listening, sending, attempting to connect, etc)"@en .

:actualGID 
			rdf:type owl:FunctionalProperty ,  owl:ObjectProperty ;
			rdfs:label "was launched by group ID"@en ;
			rdfs:domain :Process ;
			rdfs:range user:Group .

:actualUID 
			rdf:type owl:FunctionalProperty ,  owl:ObjectProperty ;
			rdfs:label "was launched by user ID"@en ;
			rdfs:domain :Process ;
			rdfs:range user:UserAccount .

:boundByProcess 
			rdf:type owl:ObjectProperty ;      
			rdfs:label "was opened by process"@en ;
			rdfs:comment "a socket must always be attached to a particular process, that will handle communications occurring over the socket and associated connection"@en ;
			rdfs:domain :Socket ;
			rdfs:range :Process ;
			owl:inverseOf :boundToIPC ,  :boundToSocket .

:boundToAddress 
			rdf:type owl:FunctionalProperty ,   owl:ObjectProperty ;
			rdfs:label "is attached to IP Address"@en ;
			rdfs:comment "a Socket must be attached to an IP Address to send and recieve information"@en ;
			rdfs:range ipnet:Address ;
			rdfs:domain :Socket .

:boundToIPC 
			rdf:type owl:ObjectProperty ;
			rdfs:label "has inter-process link"@en ;
			rdfs:comment "this process is communicating with another process via an Interprocess Communication (IPC) method"@en ;
			rdfs:range :IPC ;
			rdfs:domain :Process ;
			owl:inverseOf :boundByProcess .

:boundToSocket 
			rdf:type owl:InverseFunctionalProperty ,    owl:ObjectProperty ;
			rdfs:label "has open socket"@en ;
			rdfs:comment "identifies that this process has opened a socket (either send or receive) usually with an associated port number"@en ;
			rdfs:domain :Process ;
			rdfs:range :Socket ;
			owl:inverseOf :boundByProcess .

:currentWorkingDirectory 
			rdf:type owl:FunctionalProperty ,  owl:ObjectProperty ;
			rdfs:label "is using cuirrent working directory"@en ;
			rdfs:comment "all processes have a 'base' working directory, from which all non-absolute file paths are constructed relative to."@en ;
			rdfs:range filesystem:Directory ;
			rdfs:domain :Process .

:effectiveGID 
			rdf:type owl:FunctionalProperty ,   owl:ObjectProperty ;
			rdfs:label "is executing under effective group ID"@en ;
			rdfs:comment "if launched with sufficient privileges, a process may then relinquish those privileges by switching identity to a lesser  privileged account, usually for security purposes."@en ;
			rdfs:domain :Process ;
			rdfs:range user:Group .

:effectiveUID
			rdf:type owl:FunctionalProperty ,   owl:ObjectProperty ;
			rdfs:label "is executing under effective user ID"@en ;
			rdfs:comment "if launched with sufficient privileges, a process may then relinquish those privileges by switching identity to a lesser  privileged account, usually for security purposes."@en ;
			rdfs:domain :Process ;
			rdfs:range user:UserAccount .

:fromExecutable 
			rdf:type owl:FunctionalProperty ,   owl:ObjectProperty ;
			rdfs:label "was launched from executable file"@en ;
			rdfs:comment "this process or shared object was created from executable code loaded from the listed file."@en ;
			rdfs:range filesystem:FileName ;
			rdfs:domain :Library ,  :Process .

:hasSubProcess 
			rdf:type owl:InverseFunctionalProperty ,   owl:ObjectProperty ;
			rdfs:label "has Sub-Process"@en ;
			rdfs:comment "this process or process table has a child process"@en ;
			rdfs:subPropertyOf mere:directlyHasPart ;
			rdfs:range :Process ;
			rdfs:domain :Process ,  :ProcessList ;
			owl:inverseOf :isSubProcessOf .

:hasThread 
			rdf:type owl:FunctionalProperty ,  owl:ObjectProperty ;
			rdfs:label "has thread"@en ;
			rdfs:comment "this process has threads - simultaneously-executing portions of itself."@en ;
			rdfs:subPropertyOf mere:directlyHasPart ;
			rdfs:domain :Process , :Thread ;
			rdfs:range :Thread .

:hooksInto 
			rdf:type owl:ObjectProperty ;
			rdfs:label "hooks into"@en ;
			rdfs:range :Library ;
			rdfs:domain :Library ,  :Process .

:imports 
			rdf:type owl:ObjectProperty ;
			rdfs:label "imports"@en ;
			rdfs:comment "this process imports a shared resource (usually a code library). This link does not indicate that this process was the first to load the shared resource into memory, only that it is accessing it."@en ;
			rdfs:range :Library ;
			rdfs:domain :Process .

:isSubProcessOf 
			rdf:type owl:FunctionalProperty ,   owl:ObjectProperty ;
			rdfs:label "is Sub-Process of"@en ;
			rdfs:comment "the process that launched this process. A parent process usually has control over standard I/O of child processes and their environment variables."@en ;
			rdfs:subPropertyOf mere:directlyPartOf ;
			rdfs:range :Process ;
			rdfs:domain :Process ;
			rdfs:range :ProcessList .

:logsTo 
			rdf:type owl:ObjectProperty ;
			rdfs:label "records log to"@en ;
			rdfs:comment "indicates where a process outputs log information to - either a specific log schema object, or a simple file."@en ;
			rdfs:range log:Log ;
			rdfs:domain :Process .

:onHost 
			tapio:signaturePriority 2 ;
			rdf:type owl:FunctionalProperty ,   owl:ObjectProperty ;
			rdfs:label "is the process table from"@en ;
			rdfs:comment "Indicates the Host (the combination of hardware and OS), this process table was recorded from."@en ;
			rdfs:range host:Host ;
			owl:inverseOf host:hasProcessList ;
			rdfs:domain :ProcessList .

:openHandle 
			rdf:type owl:ObjectProperty ;
			rdfs:label "is accessing file"@en ;
			rdfs:comment "this process  is accesing a particular file, via a file handle"@en ;
			rdfs:range filesystem:FileName ;
			rdfs:domain :Process .

:boundToPort 
			rdf:type owl:DatatypeProperty ,  owl:FunctionalProperty ;
			rdfs:label "attached to port number"@en ;
			rdfs:comment "the port number this socket is connected though."@en ;
			rdfs:domain :Socket ;
			rdfs:range xsd:unsignedShort .

:commandLine 
			rdf:type owl:DatatypeProperty ,   owl:FunctionalProperty ;
			rdfs:label "command line arguments"@en ;
			rdfs:comment "the full command line (with arguments) used to invoke this process."@en ;
			rdfs:domain :Process ;
			rdfs:range xsd:string .

:displayName 
			rdf:type owl:DatatypeProperty ,   owl:FunctionalProperty ;
			rdfs:label "is identifying itself as "@en ;
			rdfs:comment "processes may include a user-friendly display name drawn from the executable that started them, that explains their functionality and origin."@en ;
			rdfs:domain :Process ;
			rdfs:range xsd:string .

:hasPID 
			tapio:signaturePriority 1 ;
			rdf:type owl:DatatypeProperty ,   owl:FunctionalProperty ;
			rdfs:label "has Process ID"@en ;
			rdfs:comment "the unique process ID number that identifies a particular instance of an executable within the process table."@en ;
			rdfs:domain :Process ;
			rdfs:range xsd:positiveInteger .

:hasSocketState 
			rdf:type owl:DatatypeProperty ,  owl:FunctionalProperty ;
			rdfs:label "socket is in state"@en ;
			rdfs:domain :Socket ;
			rdfs:range :socketState .

:processListRecorded 
			rdf:type owl:ObjectProperty , owl:FunctionalProperty ;
			rdfs:label "recorded or observed"@en ;
			rdfs:comment "linking to the event by which this process list was recorded"@en ;
			rdfs:subPropertyOf event:produced_in ;
			rdfs:domain :ProcessList;
			rdfs:range :ProcessListRecordedEvent .


:threadStarted 
			rdf:type owl:ObjectProperty , owl:FunctionalProperty ;
			rdfs:label "was  started by"@en ;
			rdfs:comment "linking to the event by which this process was  started"@en ;
			rdfs:subPropertyOf event:produced_in ;
			rdfs:domain :Thread ;
			rdfs:range :ThreadStartededEvent .

:processStarted 
			tapio:signaturePriority 3 ;
			rdf:type owl:ObjectProperty , owl:FunctionalProperty ;
			rdfs:label "was started by"@en ;
			rdfs:comment "linking to the event by which this process was started"@en ;
			rdfs:subPropertyOf event:produced_in ;
			rdfs:domain :Process ;
			rdfs:range :ProcessStartedEvent .
			
:threadEnded 
			rdf:type owl:ObjectProperty , owl:FunctionalProperty ;
			rdfs:label "was ended by"@en ;
			rdfs:comment "linking to the event by which this process was  ended"@en ;
			rdfs:subPropertyOf event:factor_of ;
			rdfs:domain :Thread ;
			rdfs:range :ThreadEndedEvent .			
:processEnded 
			rdf:type owl:ObjectProperty , owl:FunctionalProperty ;
			rdfs:label "was  ended by"@en ;
			rdfs:comment "linking to the event by which this process was ended"@en ; ;
			rdfs:subPropertyOf event:factor_of ;
			rdfs:domain :Process ;
			rdfs:range :ProcessEndedEvent .

:DatagramSocket 
			rdf:type owl:Class ;
			rdfs:label "Datagram Socket"@en ;
			rdfs:subClassOf :NetworkSocket ;
			rdfs:comment "A connectionless socket (typically used for things like the UDP Protocol)"@en .

:DomainSocket 
			rdf:type owl:Class ;
			rdfs:label "Domain Socket"@en ;
			rdfs:subClassOf :Socket ;
			rdfs:comment "A Unix Socket allows communication between two processes on the same host, similar to how a network socket allows communication between processes on different hosts. Unix Sockets typically involve the creation of a special file on the local filesystem."@en .

:DynamicLinkLibrary 
			rdf:type owl:Class ;
			rdfs:label "Dynamic Link Library"@en ;                    
			rdfs:subClassOf :Library ;                    
			rdfs:comment "the Dynamic Link Library (DLL) is commonly used in Windows Operating Systems"@en .

:IPC 
			rdf:type owl:Class ;
			rdfs:label "Inter-Process Communication"@en ;
			rdfs:subClassOf owl:Thing .

:Library 
			rdf:type owl:Class ;
			rdfs:subClassOf owl:Thing ;
			rdfs:label "Shared Executable Code Library"@en ;
			rdfs:comment "Library files contain code available for use by other processes running on the system. Typically they are .dll or .so files"@en .

:NamedPipe 
			rdf:type owl:Class ;
			rdfs:label "Named Inter-Process Communication Pipe"@en ;
			rdfs:subClassOf :Pipe ;
			rdfs:comment "A named pipe is independent of the process that created it, and may be re-used by other processes that know the name it is identified with"@en .

:NetLinkSocket 
			rdf:type owl:Class ;
			rdfs:label "NetLink Socket"@en ;
			rdfs:subClassOf :Socket ;
			rdfs:comment "Net Link Sockets are a special form of socket that enable communication between the OS Kernel itself, a a process in userspace. Often used to grant particular access to the internals of network protocol stacks. (e.g. for Firewall software)"@en .

:NetworkSocket 
			rdf:type owl:Class ;
			rdfs:label "Network Socket"@en ;
			rdfs:subClassOf :Socket .

:OrphanThread 
			rdf:type owl:Class ;
			rdfs:label "Orphaned Thread"@en ;
			rdfs:subClassOf :Thread .

:Pipe 
			rdf:type owl:Class ;
			rdfs:label "Inter-Process Pipe Connection"@en ;
			rdfs:subClassOf :IPC .

:Process 
			rdf:type owl:Class ;
			rdfs:label "Process"@en ;
			rdfs:subClassOf owl:Thing ;
			rdfs:comment "an individual process running on a host, usually with a unique process ID number associated to it, and an associated on-system executable it was instantiated from."@en .

:ProcessList 
			rdf:type owl:Class ;
			rdfs:label "Process List"@en ;
			rdfs:subClassOf owl:Thing ;
			rdfs:comment "the master process table on an execution domain (usually an instance of an operating system, but can also be a compartment within an OS)"@en .

:ProcessStartedEvent
			tapio:signaturePriority 1 ;
			rdf:type owl:Class ;
			rdfs:subClassOf event:Event ;
			rdfs:label "A process starting event"@en ;
			rdfs:comment "Starting a process."@en .
			
:ProcessEndedEvent
			rdf:type owl:Class ;
			rdfs:subClassOf event:Event ;
			rdfs:label "A process ending event"@en ;
			rdfs:comment "Ending a process."@en .	
			
:ThreadStartedEvent
			rdf:type owl:Class ;
			rdfs:subClassOf event:Event ;
			rdfs:label "A thread starting event"@en ;
			rdfs:comment "Starting a thread."@en .
			
:ThreadEndedEvent
			rdf:type owl:Class ;
			rdfs:subClassOf event:Event ;
			rdfs:label "A thread ending event"@en ;
			rdfs:comment "Ending a thread."@en .	

:ProcessListRecordingEvent
			rdf:type owl:Class ;
			rdfs:subClassOf event:Event ;
			rdfs:label "A process list recording event"@en ;
			rdfs:comment "Recording a process list on a host."@en .

:Semaphore 
			rdf:type owl:Class ;
			rdfs:label "Semaphore"@en ;
			rdfs:subClassOf :IPC ;
			rdfs:comment "A Semaphore acts as a token passed between processes, to act as a signal for which process currently has the right to acces or modify a resources, preventing collisions of two processes trying to modify the same resource simultaneously"@en .

:SharedObjectLibrary 
			rdf:type owl:Class ;
			rdfs:label "Shared Object Library"@en ;
			rdfs:subClassOf :Library ;
			rdfs:comment "Shared Object (.so) libraries are typically used by Unix-Like operating systems."@en .

:Socket 
			rdf:type owl:Class ;
			rdfs:label "Socket"@en ;
			rdfs:comment "An Inter-Process Communications Socket"@en ;
			rdfs:subClassOf owl:Thing .

:StreamSocket 
			rdf:type owl:Class ;
			rdfs:label "Stream Socket"@en ;
			rdfs:subClassOf :NetworkSocket ;
			rdfs:comment "A Connection-Based socket (typically used for things like TCP)"@en .

:Thread 
			rdf:type owl:Class ;
			rdfs:label "Thread"@en ;
			rdfs:subClassOf owl:Thing ;
			rdfs:comment "A simultaneously-executing thread within a process"@en .

:hasPriority
			rdf:type owl:DatatypeProperty, owl:FunctionalProperty ;
			rdfs:label "has priority"@en ;
			rdfs:comment "Priority is used to determine allocation of CPU resources between individual processes in a multitasking system - the higher the priority, the more CPU time a process may request"@en ;
			rdfs:domain :Process , :Thread ;
			rdfs:range xsd:decimal , xsd:normalizedString .

:hasPrivateMemoryAllocation
			rdf:type owl:DatatypeProperty, owl:FunctionalProperty ;
			rdfs:label "has total memory allocation"@en ;
			rdfs:comment "This is the total memory space requested by a a process - it may be allocated to the process from physical or virtual memory"@en ;
			rdfs:domain :Process ;
			rdfs:range xsd:unsignedLong .

:hasWorkingMemoryAllocation
			rdf:type owl:DatatypeProperty, owl:FunctionalProperty ;
			rdfs:label "has total bytes allocated in RAM"@en ;
			rdfs:comment "The Working set is the total amount of physical memory currently in use by a process, including any shared libraries and resources it is accessing."@en ;
			rdfs:domain :Process ;
			rdfs:range xsd:unsignedLong .

:hasDescription
			rdf:type owl:DatatypeProperty, owl:FunctionalProperty ;
			rdfs:label "has description"@en ;
			rdfs:comment "A free-form text description of the purpose  of this process,  usually implemented in Windows Portable Executables"@en ;
			rdfs:domain :Process ;
			rdfs:range xsd:string .

:hasCompanyName
			rdf:type owl:DatatypeProperty, owl:FunctionalProperty ;
			rdfs:label "has Company Name"@en ;
			rdfs:comment "A free-form text description of the organization that published the executable this process is an instance of, usually implemented in Windows Portable Executables"@en ;
			rdfs:domain :Process ;
			rdfs:range xsd:string .
